Add more extensive comments, and fix crash after generating error

Test/dafny0/ParseErrors.dfy
@@ -226,3 +226,23 @@ module IllegalGhost {
   ghost datatype D = D // error: cannot be 'ghost'
   ghost module M { } // error: cannot be 'ghost'
 }
+
+// ------------------------- already-ghost functions ------------------------------
+
+module AlreadyGhost {
+  // a twostate function/predicate cannot be used with ...
+  ghost twostate function F(): int { 2 } by method { } // error (x2): ... with "by method" or "ghost"
+  twostate function method G(): int { 2 } by method { } // error: ... with "by method"
+  ghost twostate predicate P() { true } by method { } // error (x2): ... with "by method" or "ghost"
+  twostate predicate method Q() { true } by method { } // error: ... with "by method"
+
+  // an extreme predicate cannot be used with ...
+  ghost least predicate I() { true } by method { } // error (x2): ... with "by method" or "ghost"
+  ghost greatest predicate J() { true } by method { } // error (x2): ... with "by method" or "ghost"
+
+  // a twostate or extreme predicate is not allowed to be declared with either "by method" or "abstract"
+  abstract twostate function A0(): int { 2 } by method { } // error (x2)
+  abstract twostate predicate A1() { true } by method { } // error (x2)
+  abstract least predicate A2() { true } by method { } // error (x2)
+  abstract greatest predicate A3() { true } by method { } // error (x2)
+}
